Add more READMEs under semantics, for #71

semantics/proofs/evaluateComputeLib.sml
@@ -1,3 +1,7 @@
+(*
+  compset for the operational semantics.
+  TODO: move up one level (cf. semanticsComputeLib)
+*)
 structure evaluateComputeLib = struct
 open HolKernel boolLib bossLib
 open semanticPrimitivesTheory evaluateTheory
